Wrote lots of comments for Base.v, stuff in Control/ and for GeneralParser.v. Rewrote the README significantly — added a section with build instructions. Implemented all functions for MonadPlus. Moved Foldable instances from Foldable.v to Instances/. Removed the old file MonadicParserCombinators.v and moved KleisliTriple.v from Misc/ to Theory/.

Control/Foldable.v
@@ -3,12 +3,14 @@ Add Rec LoadPath "/home/zeimer/Code/Coq".
 Require Export HSLib.Base.
 Require Export HSLib.Misc.Monoid.
 
-Require Import Arith.
+(** Haskell-style [Foldable]. I have no idea about the intended categorical
+    semantics. The definition is based on [foldMap] while [foldr] and [foldl]
+    are moved outside and are implemented in terms of [foldMap].
 
+    There's one law I haven't thought much about and its stated uglily
+    (a definition of monoid homomorphisms would help a lot). *)
 Class Foldable (T : Type -> Type) : Type :=
 {
-    (*foldr : forall {A B : Type}, (A -> B -> B) -> B -> T A -> B;
-    foldl : forall {A B : Type}, (B -> A -> B) -> B -> T A -> B;*)
     foldMap : forall {A : Type} {M : Monoid}, (A -> M) -> T A -> M;
     foldMap_law :
       forall (A : Type) (B C : Monoid) (f : A -> B) (g : B -> C),
@@ -16,14 +18,17 @@ Class Foldable (T : Type -> Type) : Type :=
           foldMap (f .> g) = foldMap f .> g
 }.
 
+(** A monoid instance for functions with composition and identity. It is
+    needed to define [foldr] and [foldl] using [foldMap]. *)
 Instance Endo (A : Type) : Monoid :=
 {
     carr := A -> A;
     op := @compose A A A;
     neutr := id;
 }.
-Proof. all: reflexivity. Defined.
+Proof. all: hs. Defined.
 
+(** Utility functions taken from Haskell's Data.Foldable. *)
 Section FoldableFuns.
 
 Variable A B C : Type.
@@ -31,6 +36,9 @@ Variable T : Type -> Type.
 Variable inst : Foldable T.
 Variable M : Monoid.
 
+(** Note that [foldr'], [foldl'] are not present because laziness is not a
+    problem while [foldr1] and [foldl1] are not present because the case
+    of an empty structure just cannot be omitted. *)
 Definition foldr
   {A B : Type} (f : A -> B -> B) (dflt : B) (t : T A) : B :=
     @foldMap T inst A (Endo B) (fun a : A => f a) t dflt.
@@ -52,6 +60,8 @@ Definition toListF (ta : T A) : list A :=
 
 Definition elem (cmp : A -> A -> bool) (a : A) (ta : T A) : bool :=
   foldr (fun x y => if cmp a x then true else y) false ta.
+
+Require Import Arith.
 
 Definition maxF (tn : T nat) : nat :=
   foldr (fun n m => if leb n m then m else n) 0 tn.
@@ -85,100 +95,20 @@ Definition findAll (f : A -> bool) (ta : T A) : list A :=
 
 End FoldableFuns.
 
-Arguments foldr [T inst A B] _ _ _.
-Arguments foldl [T inst A B] _ _ _.
-Arguments isEmpty [A T inst] _.
-Arguments size [A T inst] _.
-Arguments toListF [A T inst] _.
-Arguments elem [A T inst] _ _ _.
-Arguments maxF [T inst] _.
-Arguments maxBy [A T inst] _ _ _.
-Arguments minBy [A T inst] _ _ _.
-Arguments maxBy [A T inst] _ _ _.
-Arguments findFirst [A T inst] _ _.
-Arguments count [A T inst] _ _.
-Arguments findAll [A T inst] _ _.
-Arguments andF [T inst] _.
-Arguments orF [T inst] _.
-Arguments allF [A T inst] _ _.
-Arguments anyF [A T inst] _ _.
-
-Definition foldMap_Option
-  {A : Type} {M : Monoid} (f : A -> M) (oa : option A) : M :=
-match oa with
-    | None => neutr
-    | Some a => f a
-end.
-
-Instance FoldableOption : Foldable option :=
-{
-    foldMap := @foldMap_Option
-}.
-Proof.
-  intros. ext oa. destruct oa; unfold compose; cbn; congruence.
-Defined.
-
-Eval compute in isEmpty (None).
-Eval compute in size (Some 42).
-Eval compute in toListF (Some 5).
-Eval compute in elem beq_nat 2 (Some 2).
-Eval compute in maxF (Some 42).
-
-Fixpoint foldMap_List
-  {A : Type} {M : Monoid} (f : A -> M) (l : list A) :=
-match l with
-    | [] => neutr
-    | h :: t => op (f h) (foldMap_List f t)
-end.
-
-Instance FoldableList : Foldable list :=
-{
-    foldMap := @foldMap_List
-}.
-Proof.
-  intros. ext l.
-  induction l as [| h t]; unfold compose in *; cbn; congruence.
-Defined.
-
-Definition foldMap_Sum
-  {E A : Type} {M : Monoid} (f : A -> M) (x : sum E A) : M :=
-match x with
-    | inl _ => neutr
-    | inr a => f a
-end.
-
-Instance FoldableSum (E : Type) : Foldable (sum E) :=
-{
-    foldMap := @foldMap_Sum E
-}.
-Proof.
-  intros. ext x. destruct x; unfold compose; cbn; congruence.
-Defined.
-
-Eval compute in size (inr 5).
-Eval compute in maxF [1; 2; 3].
-Eval compute in findFirst (beq_nat 42) [1; 3; 5; 7; 11; 42].
-Eval compute in count (leb 10) [1; 3; 5; 7; 11; 42].
-
-Inductive BTree (A : Type) : Type :=
-    | E : BTree A
-    | T : A -> BTree A -> BTree A -> BTree A.
-
-Arguments E [A].
-Arguments T [A] _ _ _.
-
-Fixpoint foldMap_BTree
-  {A : Type} {M : Monoid} (f : A -> M) (t : BTree A) :=
-match t with
-    | E => neutr
-    | T v l r => op (f v) (op (foldMap_BTree f l) (foldMap_BTree f r))
-end.
-
-Instance FoldableBTree : Foldable BTree :=
-{
-    foldMap := @foldMap_BTree
-}.
-Proof.
-  intros. ext t.
-  induction t as [| v l IHl r IHr]; unfold compose in *; cbn; congruence.
-Defined.
+Arguments foldr {T inst A B} _ _ _.
+Arguments foldl {T inst A B} _ _ _.
+Arguments isEmpty {A T inst} _.
+Arguments size {A T inst} _.
+Arguments toListF {A T inst} _.
+Arguments elem {A T inst} _ _ _.
+Arguments maxF {T inst} _.
+Arguments maxBy {A T inst} _ _ _.
+Arguments minBy {A T inst} _ _ _.
+Arguments maxBy {A T inst} _ _ _.
+Arguments findFirst {A T inst} _ _.
+Arguments count {A T inst} _ _.
+Arguments findAll {A T inst} _ _.
+Arguments andF {T inst} _.
+Arguments orF {T inst} _.
+Arguments allF {A T inst} _ _.
+Arguments anyF {A T inst} _ _.
