Base.v
@@ -1,14 +1,25 @@
-Require Export Coq.Program.Basics.
-Require Export Coq.Logic.FunctionalExtensionality.
+(** This file is at the root of the whole library. All other files depend
+    on it. *)
 
 Require Export List.
 Export ListNotations.
 
+(** All definitions are universe polymorphic. Things are not that fine
+    however: I encountered universe inconsistencies a few times.
+
+    TODO: investigate universe consistency next time something breaks down. *)
 Global Set Universe Polymorphism.
 
-Definition id {A : Type} := fun x : A => x.
+(** Useful shorthand tactics for doing generalization and inversion. *)
+Ltac gen x := generalize dependent x.
+Ltac inv H := inversion H; subst; clear.
 
-Notation "f .> g" := (compose g f) (at level 40).
+(** We will reason by functional extensionality quite a lot. For this, we
+    have three tactics:
+    - [ext x] is a shorthand for [extensionality x]
+    - [ext] is [ext x], where x is a freshly generated name
+    - [exts] is repeated [ext] *)
+Require Export Coq.Logic.FunctionalExtensionality.
 
 Ltac ext_aux x := extensionality x.
 
@@ -17,12 +28,16 @@ Tactic Notation "ext" := let x := fresh "x" in ext x.
 
 Ltac exts := repeat ext.
 
-Ltac gen x := generalize dependent x.
+(** Program.Basics has the rest of the things we need, namely [id] and
+    [compose]. For composition, there's a forward-style notation f .> g
+    and for function application without too many parentheses there's
+    Haskell's $. *)
+Require Export Coq.Program.Basics.
 
-Ltac inv H := inversion H; subst; clear.
-
+Notation "f .> g" := (compose g f) (at level 40).
 Notation "f $ x" := (f x) (left associativity, at level 40, only parsing).
 
+(** We will need some obvious lemmas about [id]. *)
 Lemma id_eq :
   forall (A : Type) (x : A), id x = x.
 Proof. reflexivity. Qed.
@@ -41,25 +56,56 @@ Proof.
   intros. unfold compose, id. ext x. reflexivity.
 Qed.
 
+(** Our main tactics, [hs] and [monad] are based on [autorewrite] and
+    [autounfold]. These two repeatedly rewrite/unfold all things they
+    find in their hint databases. Throughout the library, we will need
+    to mark which lemmas and definitions we want rewritten/unfolded.
+
+    We need to make sure the rewriting doesn't loop and that unfolding
+    doesn't rewriting. In practice, this is very straightforward. We
+    will only add as hints those lemmas that "simplify", in some
+    subjective sense, the theorem's statement. Since rewriting is
+    performed before unfolding, we don't need to worry about it breaking
+    anything.
+
+    Both our rewriting and unfolding main hint databses are named
+    [HSLib], but there are some minor ones, like [HSLib'], [Functor]
+    and [Functor']. *)
 Hint Rewrite @id_eq @id_left @id_right : HSLib HSLib'.
 
-Definition dummy := 42.
+(** Note that rewriting and unfolding databases are separate, so we have
+    to define a dummy value and add it to the unfolding database in order
+    to initialize it. *)
+Definition the_ultimate_answer := 42.
 
-Hint Unfold dummy : HSLib HSLib'.
+Hint Unfold the_ultimate_answer : HSLib HSLib'.
 
+(** [msimpl] is the main simplification tactic we will use. We first rewrite
+    and then unfold using the rewrite/hint databases both named [HSLib].
+
+    [msimpl'] is a variant that tries to perform some simplications from
+    the hint database [HSLib'] that could result in nontermination if they
+    were added to [HSLib]. *)
 Ltac msimpl :=
   repeat (autorewrite with HSLib + autounfold with HSLib).
 
 Ltac msimpl' :=
   repeat (autorewrite with HSLib' + autounfold with HSLib).
 
+(** [hs] is a tactic for dealing with simple goals. First we try
+    [reflexivity] to make proofterms short, then we simplify and
+    at last we try [congrunce] to solve trivial equational goals.
+
+    [hs'] is a variant that uses the [msimpl'] simplification tactic
+    instead of [msimpl]. *)
 Ltac hs :=
   try split; try reflexivity; cbn; intros; msimpl; try congruence.
 
 Ltac hs' :=
   try split; try reflexivity; cbn; intros; msimpl'; try congruence.
 
-(* [destruct] on steroids that handles nested [match]es. *)
+(* [umatch] and [unmatch_all] are tactics for conveniently [destruct]ing
+    nested pattern matches. *)
 Ltac unmatch x :=
 match x with
     | context [match ?y with _ => _ end] => unmatch y
