Control/Alternative.v
@@ -3,6 +3,11 @@ Add Rec LoadPath "/home/Zeimer/Code/Coq".
 Require Export HSLib.Control.Applicative.
 Require Export HSLib.Control.Foldable.
 
+(** A Haskell-style alternative functor. The intended categorical semantics
+    is not yet entirely clear to me. Intuitively it looks like a strong
+    monoidal functor with an additional monoid structure on top of it.
+
+    The laws are standard monoid laws. *)
 Class Alternative (F : Type -> Type) : Type :=
 {
     is_applicative :> Applicative F;
@@ -23,15 +28,12 @@ Coercion is_applicative : Alternative >-> Applicative.
 
 Hint Rewrite @aplus_aempty_l @aplus_aempty_r @aplus_assoc : HSLib.
 
-Module AlternativeNotations.
-
 Notation "x <|> y" := (aplus x y)
   (left associativity, at level 50).
 
-End AlternativeNotations.
-
-Export AlternativeNotations.
-
+(** Utility functions for [Alternative]s from Haskell's
+    Control.Applicative.Alternative, Control.Applicative and Control.Monad
+    all in one place! *)
 Section AlternativeFuns.
 
 Variable F : Type -> Type.
@@ -42,13 +44,8 @@ Variable instT : Foldable T.
 
 Variables A B C : Type.
 
+(** [asum] is corresponds to Haskell's [asum], [msum] and [msum']. *)
 Definition asum : T (F A) -> F A := foldr aplus aempty.
-
-Definition aFromOption (oa : option A) : F A :=
-match oa with
-    | None => aempty
-    | Some a => pure a
-end.
 
 Fixpoint aFromList (la : list A) : F A :=
 match la with
@@ -59,6 +56,18 @@ end.
 Definition afold (ta : T A) : F A :=
   aFromList (toListF ta).
 
+Definition aFromOption (oa : option A) : F A :=
+match oa with
+    | None => aempty
+    | Some a => pure a
+end.
+
+Definition areturn (f : A -> option B) (a : A) : F B :=
+match f a with
+    | None => aempty
+    | Some b => pure b
+end.
+
 Definition optional (x : F A) : F (option A) :=
   aplus (fmap (@Some A) x) (pure None).
 
@@ -67,9 +76,10 @@ Definition guard (b : bool) : F unit :=
 
 End AlternativeFuns.
 
-Arguments asum [F instF T instT A] _.
-Arguments aFromOption [F instF A] _.
-Arguments aFromList [F instF A] _.
-Arguments afold [F instF T instT A] _.
-Arguments optional [F instF A] _.
-Arguments guard [F instF] _.
+Arguments asum {F instF T instT A} _.
+Arguments aFromList {F instF A} _.
+Arguments afold {F instF T instT A} _.
+Arguments aFromOption {F instF A} _.
+Arguments areturn {F instF A B} _ _.
+Arguments optional {F instF A} _.
+Arguments guard {F instF} _.
