README.md
@@ -2,7 +2,7 @@
 
 This project is an offshoot of my [book on Coq](https://zeimer.github.io/) (in Polish). My motivation was to find the best presentation of the concept of monad before I write about it.
 
-It then turned into a Coq library that tries to implement parts of Haskell standard library, namely Functor, Applicative, Alternative, Monad, MonadPlus, MonadTrans and maybe more. The focus is on practical functional programming and not on category theory, although all the classes come equipped with laws and instances have to obey them.
+It then turned into a Coq library that tries to implement parts of Haskell standard library. The focus is on practical functional programming and not on category theory, although (nearly) all the classes come equipped with laws and instances have to obey them.
 
 Recently I chose to write a monadic parser combinator library as a project for one (or rather, two) of my university courses. Since the parsers are monadic, they fit here perfectly. This development is based on the paper "Monadic Parser Combinators" by Graham Hutton and Erik Meijer.
 
@@ -10,50 +10,93 @@ At last, this project has great chances ending up as my BSc thesis. I'm now work
 
 ## Done
 
-The current status of the project is experimental.
+* Base.v — utilities for the whole library
+* Control/ — the core of the library. All the most important classes (Functor, Applicative, Monad etc.) live here.
+* Instances/ — types and instances for all things from Control/ besides monad transformers.
+* InstancesT/ — types and instances for monad transformers.
+* Misc/ — various things, not too interesting.
+* MonadClass/ — a directory in which classes for monad transformers are born. Nothing fancy yet.
+* MonadJoin/ — an alternative definition of monads using the join operator.
+* Parser/ — two versions of monadic parser combinators.
+* Theory/ — various theoretical results, relating applicative functors to monoidal functors, monads with bind to monads with join, kleisli triples to monads with bind and so on.
 
 Functors are a no-brainer.
 
-Applicatives come equipped with all the necessary laws and notations. Most functions that in Haskell are doubled (like liftA2 and liftM2) here come only in the Applicative version. There's also a tactic that facilitates basic reasoning with the Applicative laws. I'm also working on an equivalent characterization of Applicatives as Monoidal Functors, but this is work in progress.
+Applicatives come equipped with all the necessary laws and notations. Most functions that in Haskell are doubled (like liftA2 and liftM2) here come only in the Applicative version.
 
 Alternatives also come with notations and corresponding functions, but their laws are somewhat less polished. They are there already, but I need to think about them harder.
 
 Monads come in three flavours:
-* MonadBind — monads whose definition is based on `>>=` (bind). This is closest to the definition from the Haskell standard library.
-* MonadJoin — monads whose definition is based on `join`. This resembles the definition used in category theory.
-* MonadComp — monads whose definition is based on `>=>` (monadic composition). This definition is rare, but gives by far the best understanding of the (basic) monad laws.
+* Control.Monad — monads whose definition is based on `>>=` (bind). This is closest to the definition from the Haskell standard library and it's also the main definition used throughtout this library.
+* MonadJoin.Monad — monads whose definition is based on `join`. This resembles the definition used in category theory.
+* Theory.KleisliTriple — a weird minimalistic definition coming directly from category theory.
 
-All three flavours of Monads from this library are actually what in category theory is called monoidal monads (it's the same story as in Haskell; this is because Applicative is a superclass of Monad).
+All three flavours of Monads from this library are actually what in category theory is called monoidal monads (it's the same story as in Haskell). I have proved them all equivalent. Control.Monad and MonadJoin.Monad come equipped with all the functions one can find in Haskell standard library (well, besides `fail`) and appropriate notations, including the do-notation (although a bit retarded one).
 
-The laws for MonadBind and MonadJoin are complete now (I hope) and I have proved these two definitions equivalent. There's also a tactic that simplifies reasoning with MonadBind.
-
-MonadComp is not yet polished — it lacks some of the necessary laws (i. e. those that relate `>=>` to `fmap` and `ap`.
-
-All three definitions come equipped with all the functions one can find in Haskell standard library (well, besides `fail`) and appropriate notations, including the do-notation (although a bit retarded one).
-
-MonadPlus is there, but doesn't have any laws (besides those that come from Monad and Alternative). The functions are not there and neither are the notations.
+MonadPlus is there, but the laws are not well-thought-out (besides those that come from Monad and Alternative).
 
 Monad transformers are like in Haskell standard library and are based on the `>>=`-definition of Monad, but not yet fully worked out. The laws are there, but the classes like MonadState are lacking.
 
-Instances (Identity, Option, Sum, List, Reader, Writer, State, Cont) are defined for Functor, Applicative, Alternative and Monad whenever possible.
+For more information see the sources in Control/ — most things are a bit documented. To understand the proof style used throughtout the library, see the comments in Base.v
 
-Instances for transformers (OpionT, SumT, ReaderT, WriterT, StateT, ContT) are also defined, but there's no instance for ListT, since it doesn't obey the laws (I think).
+Instances/ contains instances for the typeclasses from Control/ for the following things: Cont, Free, Identity, Lazy (an attempt to monadiz laziness in Coq, but failed I think), list, option, prod, Reader, RoseTree, State, Sum, Writer. There's also a module All to ease importing verything at once. Note that, however, some instances for Foldable may be missing.
 
-In the directory Parser/ there are working monadic parsers combinators with Functor/Applicative/Monad instances, but they are clumsy and need to be refactored.
+InstancesT/ are instances for monad transformers and include: Codensity, ContT (along with a refactored version; ignore it), ListT (a fully working and verified one, based on the proposal "ListT Done right", but implemented using Church encoding; it even has a nice notation), OptionT, ReaderT, RoseTreeT, StateT, SumT, WriterT.
 
-Everything is compatible with Coq 8.6, but I haven't checked for 8.7.
+In the directory Parser/ there are two versions of working monadic parsers combinators with all the necessary instances: one using StateT list and the other using StateT (ListT Identity). The first one seems faster for now. There are general efficiency problems due to (I think) problems with typesclass resolution.
+
+## Build
+
+The most basic way to get things running is something along the lines of (probably, I haven't tried it myself):
+
+```
+git clone https://github.com/Zeimer/HSLib
+cd HSLib
+./rebuild.sh
+```
+
+Potential problems you may encounter:
+* permission denied — use sudo.
+* coq_makefile not found — probably your root user doesn't know where coq_makefile is. Try chown and chmod to allow your non-root user to run it.
+* ./rebuild.sh fails — a problem most likely related to CoqPath. Try COQPATH=path to HSLib on your computer.
+* incompatible version of Coq — I have tested this only for Coq 8.6 and it works, dunno about 8.7 though.
+
+A more foolproof solution is therefore:
+
+```
+sudo git clone https://github.com/Zeimer/HSLib
+sudo chown -R your_username:your_username HSLib
+sudo chmod -R u+rwx HSLib
+COQPATH=$(pwd)
+cd HSLib
+sudo ./rebuild.sh
+```
+
+You can then compile the project at any time using `make` and recompile (for example in case where you add a new file) using `./rebuild.sh`.
 
 ## TODO
 
-* Find all the necessary laws for MonadComp.
-* Prove MonadComp equivalent to MonadBind and MonadJoin.
-* Think on Alternative laws.
-* State MonadPlus laws. Define functions for MonadPlus. Take a look at the MonadPlus reform proposal.
-* Take a look at the "ListT done right proposal".
-* Take a look at other Haskell proposals relating to the standard library design.
-* Work more on Foldable.
-* Define Traversable.
-* Do something with Lazy and FreeMonad.
-* Refactor all the laws not to be point-free (point-free sucks for theorem proving.
-* Sort things out with tactics.
+The project is not over yet (and I'm not even sure if its ready to be added to OPAM). There are a few more things to be done:
+
+* Investigate universe consistency next time something breaks down. 
+* Pin down the precise categorical semantics of all classes.
+* Make sure that associativity and operator precedence are correct.
+* Find minimal sets of laws for each class.
+* Prove all the derived laws for monads (and other clases too) by hand to give an example of reasoning with monads.
+* Derive more laws.
+* Refactor all the laws not to be point-free (point-free sucks for theorem proving).
 * Try a different design in which laws come bundled in separate classes of Sort Prop.
+* State MonadPlus laws. Take a look at the MonadPlus reform proposal.
+* Take a look at other Haskell proposals relating to the standard library design.
+* Investigate commutative applicative functors and commutative monads.
+* Define Traversable and all its instances.
+* Finish proving that Applicative is equivalent to Monoidal.
+* Finish reading the paper Just Do It. Implement all the monadic classes from there are make sure they are useful for working with monad transformers.
+* Decide the existence of callCC for Codensity (I don't think it exists)
+* Decide if Codensity is commutative applicative functor.
+* Prove Codensity F isomorphic to F (?) or something like that.
+* Investigate the class for Free Monads.
+* Investigate using Church encoding for dealing with problems related to Datatypes à la carte.
+* Write reflective tactics to make proofs quicker and lighter.
+* Try to make this reflection modular using the Datatypes à la carte approach.
+* Define all instances for Foldable.
